Prove refinement of fine/coarse-grained stack

F_mu_ref_par/examples/stack/CG_stack.v
@@ -389,6 +389,23 @@ Section CG_Stack.
     repeat econstructor.
   Qed.
 
+  Definition CG_iterV (f : expr) : val :=
+    LamV (Case (Unfold (Var 1))
+              Unit
+              (
+                App (Lam (App (Var 3) (Snd (Var 2))))
+                    (App f.[ren (+3)] (Fst (Var 0)))
+              )
+        ).
+
+  Lemma CG_iter_to_val f : to_val (CG_iter f) = Some (CG_iterV f).
+  Proof. trivial. Qed.
+
+  Lemma CG_iter_of_val f : of_val (CG_iterV f) = CG_iter f.
+  Proof. trivial. Qed.
+
+  Global Opaque CG_iterV.
+
   Lemma CG_iter_closed (f : expr) :
     (∀ g, f.[g] = f) → ∀ g, (CG_iter f).[g] = CG_iter f.
   Proof. intros H g. unfold CG_iter. asimpl. rewrite ?H; trivial. Qed.
