F_mu_ref_par/examples/stack/refinement.v
@@ -5,7 +5,7 @@ From iris_logrel.F_mu_ref_par Require Import lang examples.lock
      typing logrel_binary fundamental_binary rules_binary rules.
 Import uPred.
 
-Section CG_Counter.
+Section Stack_refinement.
   Context {Σ : gFunctors} {iS : cfgSG Σ} {iI : heapIG Σ}
           {iSTK : authG lang Σ stackR}.
 
@@ -263,120 +263,259 @@ Section CG_Counter.
             rewrite -> StackLink_unfold at 2.
             iDestruct "HLK'" as {istk4 w2} "[HH [Hmpt' HLK']]".
             iDestruct "HH" as %HH'. inversion HH'; simpl in *; subst.
-            
-            iDestruct "HLK'" as "[[% %]|HLK']".
-
-            
-
-          iApply wp_value; simpl; trivial. iExists (InjLV UnitV).
-          iSplit; trivial. iLeft. iExists (_, _); repeat iSplit; simpl; trivial.
-
-
-
-
-
-
-
-
-
-
-          
-          
-          iSplitL "Hoe Hstk' HLK Hl Hstk".
-        iNext. iExists _, _, _; by iFrame "Hoe Hstk' HLK Hl Hstk".
-        clear h.
+            iDestruct (stack_mapstos_agree with "[Hmpt Hmpt']")
+              as "[Hmpt [Hmpt' %]]".
+            { by iFrame "Hmpt Hmpt'". }
+            subst.
+            iDestruct "HLK'" as "[[Heq1 Heq2]|HLK']".
+            ++ iDestruct "Heq1" as %Heq1. inversion Heq1.
+            ++ iDestruct "HLK'" as {yn1 yn2 zn1 zn2}
+                                     "[Heq1 [Heq2 [#Hrel HLK'']]]".
+               iDestruct "Heq1" as %Heq1. iDestruct "Heq2" as %Heq2.
+               inversion Heq1; subst.
+               (* Now we have proven that specification can also pop. *)
+               rewrite CG_locked_pop_of_val.
+               iPvs (steps_CG_locked_pop_suc _ _ _ _ _ _ _ _ _ _
+                     with "[Hj Hstk' Hl]") as "[Hj [Hstk' Hl]]".
+               { by iFrame "Hspec Hstk' Hl Hj". }
+               iPvsIntro. iSplitR "Hj".
+               { iNext.
+                 iClear "Hmpt Hmpt' HLK". rewrite StackLink_unfold.
+                 iDestruct "HLK''" as {istk5 w2} "[% [Hmpt HLK]]".
+                 simpl in *; subst.
+                 iExists istk5, _, _. iFrame "Hoe Hstk' Hstk Hl".
+                 rewrite StackLink_unfold.
+                 iExists _, _; iSplitR; trivial.
+                 by iFrame "HLK".
+               }
+               iApply wp_if_true. iNext.
+               iApply (@wp_bind _ _ _ [InjRCtx]); iApply wp_wand_l;
+                 iSplitR; [iIntros {w} "Hw"; iExact "Hw"|].
+               iApply wp_fst; [simpl; by rewrite ?to_of_val |
+                               simpl; by rewrite ?to_of_val |].
+               iNext. iApply wp_value; simpl.
+               { by rewrite to_of_val. }
+               iExists (InjRV _); iFrame "Hj".
+               iRight. iExists (_, _). iSplit; trivial.
+          -- (* CAS will fail *)
+            iApply (wp_cas_fail _ _ _ _ _ _ _ _ _ _ _ _ _ _).
+            iFrame "Hheap Hstk". iNext. iIntros "Hstk".
+            iSplitR "Hj".
+            { iNext. iExists _, _, _. by iFrame "Hoe Hstk' Hstk HLK Hl". }
+            iApply wp_if_false. iNext. iApply "Hlat". by iNext.
+    - (* refinement of iter *)
+      iAlways. clear j K. iIntros {j K f}. destruct f as [f1 f2]. simpl.
+      rewrite -always_later. iIntros "[#Hfs Hj]".
+      iApply wp_lam; auto using to_of_val. iNext.
+      iPvs (step_lam _ _ _ _ _ _ _ _ _ _ with "[Hj]") as "Hj".
+      { by iFrame "Hspec Hj". }
+      asimpl. rewrite FG_iter_subst CG_snap_subst CG_iter_subst. asimpl.
+      replace (FG_iter (# f1)) with (# (FG_iterV (# f1)))
+        by (by rewrite FG_iter_of_val).
+      replace (CG_iter (# f2)) with (# (CG_iterV (# f2)))
+        by (by rewrite CG_iter_of_val).
+      iApply (@wp_bind _ _ _ [AppRCtx _]); iApply wp_wand_l;
+        iSplitR; [iIntros {w} "Hw"; iExact "Hw"|].
+      iInv (N .@4) as {istk3 w h} "[Hoe [Hstk' [Hstk [HLK Hl]]]]".
+      (* coarse-grained stack takes a snapshot *)
+      iTimeless "Hstk'"; iTimeless "Hl".
+      iPvs (steps_CG_snap _ _ _ _ (K ++ [AppRCtx _]) _ _ _ _
+            with "[Hstk' Hj Hl]") as "[Hj [Hstk' Hl]]".
+      { rewrite ?fill_app. simpl. by iFrame "Hspec Hstk' Hl Hj". }
+      iApply (wp_load _ _ _ _ _ _ _).
+      iFrame "Hheap Hstk". iNext. iIntros "Hstk".
+      iDestruct (StackLink_dup with "HLK") as "[HLK HLK']".
+      iSplitR "Hj HLK'".
+      { iNext. iExists _, _, _; by iFrame "Hoe Hstk' Hstk HLK Hl". }
+      clear h.
+      rewrite ?fill_app. simpl.
+      rewrite -FG_iter_folding.
+      iRevert {istk3 w} "Hj HLK'". iLöb as "Hlat".
+      iIntros {istk3 w} "Hj". iIntros "HLK". (* A bug in iIntros? *)
+      rewrite -> FG_iter_folding at 1.
+      iApply wp_lam; simpl; trivial.
+      rewrite -FG_iter_folding. asimpl. rewrite FG_iter_subst.
+      iNext.
+      iApply (@wp_bind _ _ _ [CaseCtx _ _; LoadCtx]); iApply wp_wand_l;
+        iSplitR; [iIntros {v} "Hw"; iExact "Hw"|].
+      iApply wp_Fold; simpl; trivial.
+      iNext. simpl.
+      iApply (@wp_bind _ _ _ [CaseCtx _ _]); iApply wp_wand_l;
+        iSplitR; [iIntros {v} "Hw"; iExact "Hw"|].
+      rewrite -> StackLink_unfold at 1.
+      iDestruct "HLK" as {istk4 v} "[Heq [Hmpt HLK']]".
+      iDestruct "Heq" as %Heq. inversion Heq; subst.
+      iInv (N .@4) as {istk5 v' h} "[Hoe [Hstk' [Hstk [HLK Hl]]]]".
+      iDestruct (stack_owns_later_open_close with "[Hmpt Hoe]")
+            as "[Histk HLoe]".
+      { by iFrame "Hmpt". }
+      iApply wp_pvs.
+      iApply (wp_load _ _ _ _ _ _ _). iFrame "Hheap Histk".
+      iNext. iIntros "Histk".
+      iDestruct ("HLoe" with "[Histk]") as "[Hh Hmpt]"; trivial.
+      iDestruct "HLK'" as "[[Heq1 Heq2]|HLK']".
+      * iDestruct "Heq1" as %Heq1. inversion Heq1.
+        iDestruct "Heq2" as %Heq2. inversion Heq2.
+        rewrite CG_iter_of_val.
+        iPvs (steps_CG_iter_end _ _ _ _ _ _ _ with "[Hj]") as "Hj".
+        { by iFrame "Hspec Hj". }
+        iPvsIntro. iSplitR "Hj".
+        { iNext. iExists _, _, _. by iFrame "Hh Hstk' Hstk HLK". }
+        iApply wp_case_inl; trivial.
+        iNext. iApply wp_value; trivial. iExists UnitV. iSplitL; trivial.
+          by iSplit.
+      * iDestruct "HLK'" as {yn1 yn2 zn1 zn2}
+                              "[Heq1 [Heq2 [#Hrel HLK'']]]".
+        iDestruct "Heq1" as %Heq1. inversion Heq1.
+        iDestruct "Heq2" as %Heq2. inversion Heq2.
+        rewrite CG_iter_of_val.
+        iPvs (steps_CG_iter _ _ _ _ _ _ _ _ _ with "[Hj]") as "Hj".
+        { by iFrame "Hspec Hj". }
+        iPvsIntro. iSplitR "Hj HLK''".
+        { iNext. iExists _, _, _. by iFrame "Hh Hstk' Hstk HLK". }
+        simpl.
+        iApply wp_case_inr; simpl; rewrite ?to_of_val; trivial.
+        rewrite FG_iter_subst CG_iter_subst. asimpl.
+        iNext.
+        iApply (@wp_bind _ _ _ [AppRCtx (LamV _); AppRCtx _]);
+          iApply wp_wand_l; iSplitR; [iIntros {w'} "Hw"; iExact "Hw"|].
+        iApply wp_fst; simpl; rewrite ?to_of_val; trivial. iNext.
         iApply (@wp_bind _ _ _ [AppRCtx (LamV _)]);
-          iApply wp_wand_l; iSplitR; [iIntros {w} "Hw"; iExact "Hw"|].
-        iApply wp_Fold; simpl; auto using to_of_val.
-        iNext. iApply wp_lam; auto using to_of_val. iNext. asimpl.
-        iApply (@wp_bind _ _ _ [AppRCtx (LamV _)]);
-          iApply wp_wand_l; iSplitR; [iIntros {w} "Hw"; iExact "Hw"|].
-        iInv (N .@4) as {istk2 w h} "[Hoe [Hstk' [Hstk [HLK Hl]]]]".
-        rewrite StackLink_unfold.
-        iDestruct "HLK'" as {istk3 w2} "[Heq [Hpt HLK']]".
-        iDestruct "Heq" as %Heq. simpl in Heq; inversion Heq; subst.
-        iDestruct (stack_owns_later_open_close with "[Hpt Hoe]")
-          as "[Histk HLoe]".
-        { by iFrame "Hpt". }
-        (* Checking whether the stack is empty *)
-        iDestruct "HLK'" as "[[% %]|HLKE']".
-        * (* The stack is empty *)
-          simpl in *; subst.
-          iTimeless "Hl". iTimeless "Hstk'".
-          iPvs (steps_CG_locked_pop_fail _ _ _ _ _ _ _ _ with "[Hj Hstk' Hl]")
-            as "[Hj [Hskt' Hl]]".
-          { iFrame "Hspec Hstk' Hl Hj". }
-          iApply (wp_load _ _ _ _ _ _ _). iFrame "Hheap Histk".
-          iNext. iIntros "Histk".
-          
-          iSplitR "Hj".
-          { iNext. iExists _, _, _. iFrame "Hstk' Hstk HLK Hl".
-            iDestruct ("HLoe" with "[Histk]") as "[Hh _]"; trivial.
-          }
-        iApply wp_lam; auto using to_of_val. iNext.
-        asimpl.
-        
+          iApply wp_wand_l; iSplitR; [iIntros {w'} "Hw"; iExact "Hw"|].
+        rewrite -> StackLink_unfold at 1.
+        iDestruct "HLK''" as {istk6 w'} "[% HLK]".
+        simpl in *; subst.
+        iSpecialize ("Hfs" $! _ (K ++ [AppRCtx (LamV _)]) (yn1, zn1)).
+        rewrite fill_app; simpl.
+        iApply wp_wand_l; iSplitR "Hj"; [|iApply "Hfs"; by iFrame "Hrel Hj"].
+        iIntros {u}; simpl.
+        iIntros "Hj". iDestruct "Hj" as {z} "[Hj [% %]]".
+        rewrite fill_app; simpl. subst. asimpl.
+        iPvs (step_lam _ _ _ _ _ _ _ _ _ _ with "[Hj]") as "Hj".
+        { by iFrame "Hspec Hj". } asimpl. rewrite CG_iter_subst. asimpl.
+        replace (CG_iter (# f2)) with (# (CG_iterV (# f2)))
+          by (by rewrite CG_iter_of_val).
+        iPvs (step_snd _ _ _ _ (K ++ [AppRCtx _]) _ _ _ _ _ _ _ with "[Hj]")
+          as "Hj".
+        { rewrite fill_app; simpl. by iFrame "Hspec Hj". }
+        rewrite fill_app; simpl.
+        iApply wp_lam; simpl; trivial.
+        iNext. rewrite FG_iter_subst. asimpl.
+        replace (FG_iter (# f1)) with (# (FG_iterV (# f1)))
+          by (by rewrite FG_iter_of_val).
+        iApply (@wp_bind _ _ _ [AppRCtx _]);
+          iApply wp_wand_l; iSplitR; [iIntros {w''} "Hw"; iExact "Hw"|].
+        iApply (wp_snd _ _ _ _ _ _); auto using to_of_val.
+        simpl. iNext. rewrite -FG_iter_folding.
+        iSpecialize ("Hlat" $! istk6 zn2).
+        iApply ("Hlat" with "[Hj] [HLK]"); trivial.
+        rewrite -> StackLink_unfold at 2.
+        iExists _, _; iSplitR; trivial.
+        Unshelve.
+        all: try match goal with
+                   |- to_val _ = _ => simpl; by rewrite ?to_of_val
+                 end.
+        all: trivial.
+        all: try match goal with
+                   |- _ ≠ _ => let H := fresh "H" in intros H; inversion H; auto
+                 end.
+        (* This seems to be a bug in all: mechanism!? *)
+        match goal with
+          |- @subseteq
+              _ _ (nclose (N .@ ?A))
+              (@difference _ _ ⊤ (nclose (N .@ ?B))) =>
+          abstract (prove_disj N A B)
+        end.
+        match goal with
+          |- @subseteq
+              _ _ (nclose (N .@ ?A))
+              (@difference _ _ ⊤ (nclose (N .@ ?B))) =>
+          abstract (prove_disj N A B)
+        end.
+        match goal with
+          |- @subseteq
+              _ _ (nclose (N .@ ?A))
+              (@difference _ _ ⊤ (nclose (N .@ ?B))) =>
+          abstract (prove_disj N A B)
+        end.
+        match goal with
+          |- @subseteq
+              _ _ (nclose (N .@ ?A))
+              (@difference _ _ ⊤ (nclose (N .@ ?B))) =>
+          abstract (prove_disj N A B)
+        end.
+        match goal with
+          |- @subseteq
+              _ _ (nclose (N .@ ?A))
+              (@difference _ _ ⊤ (nclose (N .@ ?B))) =>
+          abstract (prove_disj N A B)
+        end.
+        match goal with
+          |- @subseteq
+              _ _ (nclose (N .@ ?A))
+              (@difference _ _ ⊤ (nclose (N .@ ?B))) =>
+          abstract (prove_disj N A B)
+        end.
+        match goal with
+          |- @subseteq
+              _ _ (nclose (N .@ ?A))
+              (@difference _ _ ⊤ (nclose (N .@ ?B))) =>
+          abstract (prove_disj N A B)
+        end.
+        match goal with
+          |- @subseteq
+              _ _ (nclose (N .@ ?A))
+              (@difference _ _ ⊤ (nclose (N .@ ?B))) =>
+          abstract (prove_disj N A B)
+        end.
+        match goal with
+          |- @subseteq
+              _ _ (nclose (N .@ ?A))
+              (@difference _ _ ⊤ (nclose (N .@ ?B))) =>
+          abstract (prove_disj N A B)
+        end.
+        match goal with
+          |- @subseteq
+              _ _ (nclose (N .@ ?A))
+              (@difference _ _ ⊤ (nclose (N .@ ?B))) =>
+          abstract (prove_disj N A B)
+        end.
+        match goal with
+          |- @subseteq
+              _ _ (nclose (N .@ ?A))
+              (@difference _ _ ⊤ (nclose (N .@ ?B))) =>
+          abstract (prove_disj N A B)
+        end.
+        match goal with
+          |- @subseteq
+              _ _ (nclose (N .@ ?A))
+              (@difference _ _ ⊤ (nclose (N .@ ?B))) =>
+          abstract (prove_disj N A B)
+        end.
+        match goal with
+          |- @subseteq
+              _ _ (nclose (N .@ ?A))
+              (@difference _ _ ⊤ (nclose (N .@ ?B))) =>
+          abstract (prove_disj N A B)
+        end.
+        match goal with
+          |- @subseteq
+              _ _ (nclose (N .@ ?A))
+              (@difference _ _ ⊤ (nclose (N .@ ?B))) =>
+          abstract (prove_disj N A B)
+        end.
+        match goal with
+          |- @subseteq
+              _ _ (nclose (N .@ ?A))
+              (@difference _ _ ⊤ (nclose (N .@ ?B))) =>
+          abstract (prove_disj N A B)
+        end.
+        match goal with
+          |- @subseteq
+              _ _ (nclose (N .@ ?A))
+              (@difference _ _ ⊤ (nclose (N .@ ?B))) =>
+          abstract (prove_disj N A B)
+        end.
+  Qed.
 
-
-        iApply (@wp_bind _ _ _ [IfCtx _ _; CasRCtx (LocV _) (FoldV (LocV _));
-                                FoldCtx]);
-          iApply wp_wand_l; iSplitR; [iIntros {w} "Hw"; iExact "Hw"|].
-        iApply wp_alloc; simpl; trivial; [by rewrite to_of_val|].
-        iFrame "Hheap". iNext. iIntros {ltmp} "Hltmp".
-        iApply (@wp_bind _ _ _ [IfCtx _ _]);
-          iApply wp_wand_l; iSplitR; [iIntros {w} "Hw"; iExact "Hw"|].
-        iInv (N .@4) as {istk2 v h} "[Hoe [Hstk' [Hstk [HLK Hl]]]]".
-        (* deciding whether CAS will succeed or fail *)
-        destruct (decide (istk = istk2)) as [|Hneq]; subst.
-        * (* CAS succeeds *)
-          (* In this case, the specification pushes *)
-          iTimeless "Hstk'". iTimeless "Hl".
-          iPvs (steps_CG_locked_push _ _ _ j K _ _ _ _ _ with "[Hj Hl Hstk']")
-            as "[Hj [Hstk' Hl]]".
-          { rewrite CG_locked_push_of_val. by iFrame "Hspec Hstk' Hj". }
-          iApply wp_pvs.
-          iApply (wp_cas_suc _ _ _ _ _ _ _ _ _ _ _); simpl; trivial.
-          iFrame "Hheap Hstk". iNext. iIntros "Hstk".
-          iSplitR "Hj".
-          { iPvs (stack_owns_alloc with "[Hoe Hltmp]") as "[Hoe Hpt]".
-            { by iFrame "Hoe". }
-            iPvsIntro. iNext. iExists ltmp, _, _.
-            iFrame "Hoe Hstk' Hstk Hl".
-            do 2 rewrite StackLink_unfold.
-            rewrite -StackLink_unfold.
-            iExists _, _. iSplit; trivial.
-            iFrame "Hpt". iRight. iExists _, _, _, _.
-            repeat iSplitR; trivial.
-            iNext; trivial.
-          }
-          iPvsIntro.
-          iApply wp_if_true. iNext; iApply wp_value; trivial.
-          iExists UnitV. iFrame "Hj"; by iSplit.
-        * iApply (wp_cas_fail _ _ _ _ _ _ _ _ _ _ _ _ _ _); simpl; trivial.
-          iFrame "Hheap Hstk". iNext. iIntros "Hstk".
-          iSplitR "Hj".
-          { iNext. iExists _, _, _. by iFrame "Hoe Hstk' Hstk Hl". }
-          iApply wp_if_false. iNext. iApply "Hlat". by iNext.
-
-
-
-
-
-
-
-
-
-
-
-
-
-
-
-
-
-
-
-
-
-
-        
+End Stack_refinement.
